F* forgets recursive function's post-condition???
The insert function has is_bst as postcondition.
I expect to get this postcondition when calling insert recursivelly.
But apparently I don't.

examples/data_structures/binary_search_tree_basic.fst
@@ -1,19 +1,19 @@
 module BinarySearchTreeBasic
 
 type tree =
-  | Leaf : n:int -> tree
+  | Leaf : tree
   | Node : n:int -> tree -> tree -> tree
 
 val in_tree : int -> tree -> Tot bool
 let rec in_tree x t =
   match t with
-  | Leaf n -> x = n
+  | Leaf n -> false
   | Node n t1 t2 -> x = n || in_tree x t1 || in_tree x t2
 
 val all : (int -> Tot bool) -> tree -> Tot bool
 let rec all p t =
   match t with
-  | Leaf n -> p n
+  | Leaf n -> true
   | Node n t1 t2 -> p n && all p t1 && all p t2
 
 (* CH: don't these already have some non-operator form? *)
@@ -40,7 +40,21 @@ let rec aux p x t =
 val search : x:int -> t:tree{is_bst t} -> Tot (r:bool{r <==> in_tree x t})
 let rec search x t =
   match t with
-  | Leaf n -> x = n
+  | Leaf n -> false
   | Node n t1 t2 -> if x = n then      true
                     else if x < n then search x t1
                     else               search x t2
+
+val insert : x:int -> t:tree -> Pure tree
+               (requires (is_bst t))
+               (ensures (fun r -> is_bst r /\
+                 (forall y. in_tree y r <==> (in_tree y t \/ x = y))))
+let rec insert x t =
+  match t with
+  | Leaf -> Node x Leaf Leaf
+  | Node n t1 t2 -> if x = n then      t
+                    else if x < n then
+                      (assert (is_bst (insert x t1)); (* WTF? *)
+                       admit() (*Node n (insert x t1) t2*))
+                    else
+                      admit()(*Node n t1 (insert x t2)*)
